<?xml version="1.0" encoding="UTF-8" ?>
<section xml:id="derivatives-of-compositions-chain-rule">
<title>Derivatives of compositions: chain rule</title>


<paragraphs xml:id="the-plan-11">
<title>The Plan</title>

<p> We will encounter our most powerful method for computing
derivatives, the chain rule.<!-- linebreak -->
</p>


<paragraphs xml:id="many-derivatives">
<title>Many derivatives</title>

<p>	We now know how to find derivatives of sums of
polynomial terms, exponential functions, or natural logarithms. In
addition to products and quotients (next time), we can also combine
functions using .
</p>


<paragraphs xml:id="the-art-of-compositions">
<title>The <sq>art</sq> of compositions</title>

<p> It helps to think of a function <m>h(x)=(f\circ g)(x)=f(g(x))</m>,
as being <sq>built</sq> from two component functions
<m>f</m> and <m>g</m> using function composition.
</p>

<table>
<title></title>
<tabular>
<row header="yes">
<cell halign="left">Label</cell>
<cell halign="left">Interpretation</cell>
<cell halign="left">Identification (Tips)</cell>
</row>
<row class="odd">
<cell halign="left"></cell>
<cell halign="left"></cell>
<cell halign="left"></cell>
</row>
<row class="even">
<cell halign="left"><m>h(x)</m></cell>
<cell halign="left"></cell>
<cell halign="left"></cell>
</row>
<row class="odd">
<cell halign="left"><m>g(x)</m></cell>
<cell halign="left"></cell>
<cell halign="left"></cell>
</row>
<row class="even">
<cell halign="left"><m>f(g)</m></cell>
<cell halign="left"></cell>
<cell halign="left"></cell>
</row>
</tabular>
</table>

<p> The function <m>F(x)=e^{-x^{2}}</m> is a
composition of the  function <m>f(g)=e^g</m> with the  function
<m>g(x)=-x^{2}</m>.
</p>

<p> The function <m>f(z)=\ln{(z^{3}-z)}</m> is the
composition of which two functions?
</p>

<p> The function
<m>H(y)=\displaystyle\frac{1}{1+y^{2}}</m> is the composition of which
two
functions?
</p>

<p> Suppose <m>h(x)=(f\circ g)(x)=f(g(x))</m>, where
<m>f</m> and <m>g</m> are both differentiable functions. Then
<me>\boxed{h'(x)=f'(g(x))g'(x) \qquad \textrm{or} \qquad
\displaystyle\frac{dh}{dx}=\frac{df}{dg}\frac{dg}{dx}}</me>
</p>

<p> To use the chain rule,
</p>

<p><ol>
<li> <p> write the function as a composition<!--
linebreak --></p> </li>
<li> <p> take the derivatives of the component pieces<!--
linebreak --></p> </li>
<li> <p> multiply the derivatives together, giving the
product the appropriate name<!-- linebreak --></p> </li>
<li> <p> put everything back in terms of the original
variable<!-- linebreak --></p> </li>

</ol></p>

<p> Find the derivative of <m>F(x)=e^{-x^{2}}</m>.
</p>

<p> Find the derivative of <m>f(z)=\ln{(z^{3}-z)}</m>.
</p>

<p> Find the derivative of
<m>H(y)=\displaystyle\frac{1}{1+y^{2}}</m>.
</p>

<p> Find the derivative of <m>h(x)=e^{cx}</m>.
</p>

</paragraphs>

<paragraphs xml:id="hint">
<title>Hint</title>

<p> In some instances, it may be easier to use the
chain rule by identifying an <q>outer function</q> and an <q>inner
function</q> than it is to <term>explicitly</term> apply the algorithm.
The derivative of the composition is then the derivative of the outer
function times the derivative of the inner function.
</p>

<p> Find the derivative of
<m>h(t)=(17+4t+5t^{2}+3t^{3})^{2}</m>.
</p>

<p> Find the derivative of <m>v(x)=e^{2x^{3}}</m>.
</p>

<p> Find the derivative of
<m>h(y)~=~\ln(y^{2}+2y+1)</m>.
</p>

<p> Find the derivative of <m>F(x)=(2x^{2}+3x)^{4}</m>.
</p>

</paragraphs>

<paragraphs
xml:id="implicit-differentiation-and-related-rates">
<title>Implicit differentiation and Related
rates</title>

<p> Even when we do not have a formula for a
function, we can still study its derivatives by invoking the chain rule.
Many classic problems tend to be based on geometric relationships
between two variables.
</p>

</paragraphs>

<paragraphs
xml:id="do-we-have-any-more-time-for-related-rates">
<title>Do we have any more time for related
rates?</title>

<p> If so, let’s try a classic calculus problem. If
not, check online for a supplemental handout.
</p>

</paragraphs>
</paragraphs>
</paragraphs>

<exercises xml:id="quick-practice-chain" class="unnumbered">
<title>Quick practice</title>


<exercise><statement> <p> What is the derivative of <m>f(x) =
(3x-7)^{2}</m>?</p> </statement>
<solution>
<p> The derivative of <m>f(x) = (3x-7)^{2}</m> is <m>f'(x) =
2(3x-7)(3) = 6(3x-7) = 18x-42</m>.</p>
</solution>
</exercise>

<exercise><statement> <p> (This one might not be so quick practice.)
Recall <m>E =
aM^b</m> discussed earlier in the context of applications of exponential
and logarithmic functions. This time assume that <m>E</m> and <m>M</m>
change with respect to time, for example in a growing animal, and that
<m>a</m> and <m>b</m> are parameters (particular numbers, but in this
fashion using a letter as a placeholder so we do not have to worry about
the value of the number itself). Together this all means that <m>E(t) =
aM(t)^b</m>. Using the chain rule, compute the derivative
<m>E'(t)</m>.</p> </statement>
<solution>
<p> Though we don’t know the exact formula for <m>E(t)</m>
we can still apply the reasoning behind the chain rule. In fact,
<me>E'(t) = abM(t)^{b-1}M'(t)</me></p>
</solution>
</exercise>

</exercises>
</section>
<!-- ******************************* -->