<?xml version="1.0" encoding="UTF-8" ?>

<section xml:id="applications-to-chemistry">
<title>Applications to chemistry</title>


<paragraphs xml:id="the-plan-18">
<title>The Plan</title>

<p> We continue our work on integration by introducing an
application to autonomous differential equations via the integrated rate
laws - a cornerstone of chemical kinetics.
</p>


<paragraphs xml:id="background">
<title>Background</title>
<p>The <term>integrated rate laws</term> exist at the interface of
calculus and chemistry.  By studying these equations from a calculus
perspective, the results are much more cohesive than it might first
appear.  Often "we" are interested in the change in concentration of a
particular chemical species.  Here let, <me> A(t) = [A]_{t} = [A] \text{
at time }t =\text{ concentration of species }A\text{ at time }t.</me> To be
consistent with class notation and objectives, we will use <m>A(t)</m> 
to refer to the concentration.
</p>

<paragraphs xml:id="zeroth-order">
<title>Zeroth order</title> <p>Within this family, the first formula
comes from the zeroth order reaction given by <me>\dfrac{dA}{dt} =
-kA^0.</me> Since this contains <m>A^0 = 1</m>, the right-hand side simplifies to
the constant <m>-k</m>.  At this point, we are looking for an unknown
function <m>A(t)</m> whose derivative is the constant <m>-k</m>. Thinking
about this from the perspective of differentiation, we are looking for a
function <m>A(t)</m> whose derivative is a constant.  This means that is
linear and that constant, <m>-k</m>, is its slope. So, <me>
A(t) = -kt+A_{0},</me> where <m>A_{0}</m> is the <term>constant of
integration</term> and gives the initial concentration of the reactant. </p>

<!--><p>This turns out to be one of the simplest, most useful, but also most
cleverly disguised applications of the technique of <term>integration by
<m>u</m>-substitution</term>. Our goal is to put the <m>A</m>-like
variables on the left and leave everything <em>else</em> on the
right-hand side and immediately integrate with respect to time <m>t</m>.
 This results in <me> \begin{aligned}[t] \dfrac{dA}{dt} \amp = -k A^{0}\\
\dfrac{dA}{dt} \amp = -k\\
\int\dfrac{dA}{dt}\,dt \amp = \int -k\, dt \end{aligned}
</me> </p>
-->
<!--><p>This is somewhat abstract, but we can immediately apply
<m>u</m>-substitution.  To do so, we have to recognize that the unknown
function is <m> u = A(t)</m> and that <me> du = A'(t)\,dt</me>. Now,
this isn't immediately useful, but remembering our notation <me>A'(t) =
\dfrac{dA}{dt}</me>, so we can write, <me>du = \dfrac{dA}{dt}\,dt</me>.
Suddenly we are finished with our process of <m>u</m>-substittution and
can integrate.  Continuing from above <me> \begin{aligned}[t]
\int\underbrace{\frac{1}{A}}_{\frac{1}{u}}\cdot\underbrace{\frac{dA}{
dt}\,dt}_{du} \amp = \int -k\, dt\\ \int \frac{1}{u}\,du \amp = \int
-k\,dt\\ \ln|u| \amp = -kt+c \end{aligned} </me> </p>-->

<!--><p>Remembering above that <m>u = A(t)</m> we can return to our chemistry
notation, that <me>\ln|A(t)| = -kt+c</me>.  What is left is to specify a
value for <m>c</m>. Thinking of our physical situation we have that
<m>A(0) = A_{0}</m> (again as a chemist you might be picturing the
 quantity <m>[A]_{0}</m>, but this bracket notation is somewhat
 unsatisfying mathematically).  This gives <me>\ln|A(0)| = \ln|A_{0}| =
 -k(0) + c</me>, or <m>c = \ln|A_{0}|</m>. Since we expect <m>A_{0} \gt
 0</m>, we can neglect the absolute value bars in favor of notational
 simplicity. This gives the <term>zeroth-order integrated rate
 law</term>, <me> \ln(A_{0}) = -kt+A_{0}</me>. Under these assumptions
 we expect the concentration fo chemical species <m>A</m> to decay linearly as a 
 function of time with a slope of <m>-k</m>, beginning from an initial
 concentration of <m>A_{0}</m>.</p>-->

<!--><p>In what follows the higher order integrated rate law formulas are
obtained with the same approach - integration.  The only thing that separates
remaining cases from the first is the power on the concentration
<m>A = A(t)</m> on the right-hand side of the original differential equation.
This influences how the details of integration play out, but really
nothing more.</p>-->

</paragraphs>

<paragraphs xml:id="first-order">
<title>First order</title>
<p>Since the differential equation is <me>\dfrac{dA}{dt} = -kA</me>, we
can <em>guess</em> the solution by answering the question, "what
function has a derivative that is a constant times itself?".  Since
<me>\dfrac{d}{dt}\left(e^{-kt}\right) = -ke^{-kt}</me>, It turns
out that multiplying by a constant we have
<me>\dfrac{d}{dt}\left(A_{0}e^{-kt}\right) = -A_{0}ke^{-kt} =
-k\underbrace{A_{0}e^{-kt}}_{A(t)}</me>
</p>
</paragraphs>

<paragraphs xml:id="first-order-revisited">
<title>First order - revisited</title>

<p>Just like before, but now with a power of <m>n = 1</m> on the
right-hand side, we have <me>\dfrac{dA}{dt} \amp = -k A</me>. Our goal
will be to move all of the <m>A</m>-like quantities to the left-hand
side and leave any constants on the right-hand side.  This turns out to
give some evidence in support of a well-known technique in differential
equations called <em>separation of variables</em>.  We proceed as
follows, first dividing by <m>A</m> on each side, then integrating each
side with respect to <m>t</m>,
<me>\begin{aligned}[t] \dfrac{dA}{dt} \amp = -k A\\
\dfrac{1}{A}\cdot\dfrac{dA}{dt} \amp = -k\\ 
\int \dfrac{1}{A}\cdot\dfrac{dA}{dt}\,dt \amp = \int -k\, dt \end{aligned}
</me> </p>

<p>This is somewhat abstract, but we can immediately apply
<m>u</m>-substitution.  To do so, we have to recognize that the unknown
function is <m> u = A(t)</m> and that <me> du = A'(t)\,dt</me>. Now,
this isn't immediately useful, but remembering our notation <me>A'(t) =
\dfrac{dA}{dt}</me>, so we can write, <me>du = \dfrac{dA}{dt}\,dt</me>.
Suddenly we are finished with our process of <m>u</m>-substittution and
can integrate.  Continuing from above <me> \begin{aligned}[t]
\int\underbrace{\frac{1}{A}}_{\frac{1}{u}}\cdot\underbrace{\frac{dA}{
dt}\,dt}_{du} \amp = \int -k\, dt\\ \int \frac{1}{u}\,du \amp = \int
-k\,dt\\ \ln|u| \amp = -kt+c \end{aligned} </me> </p>

<p>Remembering above that <m>u = A(t)</m> we can return to our chemistry
notation, that <me>\ln|A(t)| = -kt+c</me>.  What is left is to specify a
value for <m>c</m>. Thinking of our physical situation we have that
<m>A(0) = A_{0}</m> (again as a chemist you might be picturing the
 quantity <m>[A]_{0}</m>, but this bracket notation is somewhat
 unsatisfying mathematically).  This gives <me>\ln|A(0)| = \ln|A_{0}| =
 -k(0) + c</me>, or <m>c = \ln|A_{0}|</m>. Since we expect <m>A_{0} \gt
 0</m>, we can neglect the absolute value bars in favor of notational
 simplicity. This gives the <term>zeroth-order integrated rate
 law</term>, <me> \ln(A(t)) = -kt+\ln(A_{0})</me>. Under these assumptions
 we expect the concentration of chemical species <m>A</m> to decay linearly as a 
 function of time with a slope of <m>-k</m>, beginning from an initial
 concentration of <m>A_{0}</m>.</p>
 
 <p>In this case, the plot of the natural logarithm of the observed
 concentration will resemble a decreasing linear function.</p>
 
<p>We may also be aware that a first-order reaction corresponds to
<term>exponential decay</term>, in fact, exponentiating both sides of
the formula above gives <me>\begin{aligned}[t]
\ln(A(t)) \amp = -kt+\ln(A_{0})\\
e^{\ln(A(t))} \amp = e^{-kt+\ln(A_{0})}\\
A(t) \amp = e^{-kt}\cdot e^{\ln(A_{0})}\\
A(t) \amp = e^{-kt}A_{0}\\
A(t) \amp = A_{0}e^{-kt}\\
\end{aligned}</me>
</p>

<p>Historically it was important to express data in terms of linear
relationships, so a plot of the natural logarithm of a measurement that
gave rise to a linear trend was a good indicator of this relationship
and estimation of the slope <m>k</m> was relatively easy.  In contemporary times
it is relatively easy to 'fit' nonlinear functions like exponentials, so
it would be reasonable to plot the raw data, not its natural logarithm,
and look the underlying exponential relationship and its parameter
<m>k</m>.</p> </paragraphs>

<paragraphs xml:id="second-order">
<title>Second order</title>
<p>Just like before, but now with a power of <m>2</m> on the right-hand
side <me> \begin{aligned}[t] \dfrac{dA}{dt} \amp = -k A^{2}\\
\dfrac{1}{A^2}\cdot\dfrac{dA}{dt} \amp = -k\\ \int
A^{-2}\cdot\dfrac{dA}{dt}\,dt \amp = \int -k\, dt \end{aligned}
</me> </p>

<p>Again the unknown
function is <m> u = A(t)</m> and that <me> du = A'(t)\,dt</me>. Now,
this isn't immediately useful, but remembering our notation <me>A'(t) =
\dfrac{dA}{dt}</me>, so we can write, <me>du = \dfrac{dA}{dt}\,dt</me>.
Suddenly we are finished with our process of <m>u</m>-substittution and
can integrate.  Continuing from above <me> \begin{aligned}[t]
\int\underbrace{A^{-2}}_{u^{-2}}\cdot\underbrace{\frac{dA}{
dt}\,dt}_{du} \amp = \int -k\, dt\\ \int u^{-2}\,du \amp = \int
-k\,dt\\
\left(\frac{1}{-2+1}\right)u^{-2+1} \amp = -kt+c\\
-u^{-1}\amp = -kt+c\\
-\frac{1}{u}\amp = -kt+c\\
-\frac{1}{A(t)}\amp = -kt+c\\
 \end{aligned} </me>
 Using the initial condition, <me>-\frac{1}{A(0)} = -\frac{1}{A_{0}} =
 -k(0) + c</me> or <m>c = -\frac{1}{A_{0}}</m>
</p>
<p>Solving for <m>A(t)</m> we have 
<me> \begin{aligned}[t]
-\frac{1}{A(t)}\amp = -kt-\frac{1}{A_{0}}\\
\frac{1}{A(t)}\amp = kt+\frac{1}{A_{0}}\\
A(t)\amp = \frac{1}{kt+A_{0}}\\
 \end{aligned} </me></p>
 
 <p>The plot of the reciprocal of <m>A(t)</m> is an increasing linear
 function with a slope of <m>k \gt 0</m>.
 </p>
</paragraphs>

<paragraphs xml:id="summary">
<title>Summary</title>
<p>Three very different looking formulas 
<me> \begin{aligned}[t]
\text{zeroth order: }\amp A(t) = -kt + A_{0}\\
\text{first order: }\amp \ln(A(t)) = -kt + \ln(A_{0})\\
\text{second order: }\amp \frac{1}{A(t)} = kt + \frac{1}{A_{0}}
\end{aligned} </me>
all result from integration of
<me>\dfrac{dA}{dt} = -kA^n</me> for different values of <m>n</m>
corresponding to the reaction order.  Solving each for <m>A(t)</m>
suggests that <m>A(t)</m> evolves very differently in each case.</p>
</paragraphs>
</paragraphs>
</paragraphs>

<exercises xml:id="quick-practice-chemistry" class="unnumbered">
<title>Quick practice</title>

</exercises>

</section>